Fix join

syntax.sig
@@ -13,3 +13,4 @@ tBool : tm
 tEq : tm -> tm -> tm -> tm
 tJ : tm -> tm -> tm -> tm -> tm
 tRefl : tm
+tProp : tm
