imports.v
@@ -5,3 +5,4 @@ From Equations Require Export Equations.
 From Hammer Require Export Tactics.
 From stdpp Require Export relations (rtc, rtc_transitive, rtc_once, rtc_inv, rtc(..), diamond, confluent, diamond_confluent).
 Require Export Psatz.
+Require Export Setoid.
